StVM.v
@@ -1,0 +1,12 @@
+Require Import MyStack ConcreteEvidence.
+Require Import Maps.
+
+(* Specific VM monad *)
+Definition ev_stack := gen_stack EvidenceC.
+Definition ev_store := Map nat EvidenceC.
+Record vm_st : Type := mk_st
+                         {st_ev:EvidenceC ;
+                          st_stack:ev_stack ; 
+                          st_trace:list Ev ;
+                          st_pl:Plc ;
+                          st_store:ev_store}.
